vendor/record-update/RecordSet.v
@@ -98,8 +98,14 @@ Hint Extern 1 (SetterWf _) => SetterWfInstance_t : typeclass_instances.
 Module RecordSetNotations.
   Delimit Scope record_set with rs.
   Open Scope rs.
-  Notation "x <| proj  :=  v |>" := (set proj (constructor v) x)
+  Notation "x <| proj  :=  v |>" := (set proj (fun _ => v) x)
                                     (at level 12, left associativity) : record_set.
   Notation "x <| proj  ::=  f |>" := (set proj f x)
                                      (at level 12, f at next level, left associativity) : record_set.
+  Notation "x <| proj1 ; proj2 ; .. ; projn := v |>" :=
+    (set proj1 (set proj2 .. (set projn (fun _ => v)) ..) x)
+    (at level 12, left associativity).
+  Notation "x <| proj1 ; proj2 ; .. ; projn ::= f |>" :=
+    (set proj1 (set proj2 .. (set projn f) ..) x)
+    (at level 12, left associativity).
 End RecordSetNotations.
